projects/pbarenbaum/SDRS.v
@@ -27,47 +27,87 @@ Structure ARS := mkARS {
 Definition term {A} := ars_term A.
 Definition step {A} := ars_step A.
 
-(* Finite reduction sequences *)
-Inductive finreduction {A : ARS} :
-  forall t s : @term A, Type :=
-    | id     : forall {t : term}, finreduction t t
-    | frcons : forall {t1 t2 t3 : term},
-                 step t1 t2 ->
-                 finreduction t2 t3 ->
-                 finreduction t1 t3.
+Definition step_src {A} {s t : @term A} (u : step s t) : term := s.
+Definition step_tgt {A} {s t : @term A} (u : step s t) : term := t.
 
-Fixpoint finreduction_length {A : ARS} {s t : @term A}
-                             (P : finreduction t s) : nat :=
-  match P with
-  | id          => O
-  | frcons _ P' => S (finreduction_length P')
-  end.
+Section FiniteReductionSequences.
 
-Fixpoint finreduction_append {A : ARS} {t1 t2 t3 : @term A}
-                             (P : finreduction t1 t2) :
-                             finreduction t2 t3 -> finreduction t1 t3 :=
-  match P with
-  | id          => fun Q => Q
-  | frcons u P' => fun Q => frcons u (finreduction_append P' Q)
-  end.
+    (* Finite reduction sequences ("cons" representation) *)
+    Inductive finreduction {A : ARS} :
+      forall t s : @term A, Type :=
+        | id     : forall {t : term}, finreduction t t
+        | frcons : forall {t1 t2 t3 : term},
+                     step t1 t2 ->
+                     finreduction t2 t3 ->
+                     finreduction t1 t3.
 
-Section ReductionExample.
-    Variable A : ARS.
-    Variable t : @term A.
-    Variable ua ub uc ud ue uf : step t t.
-    Check id.
-    Check frcons ua id.
-    Check frcons ua (frcons ub id).
-    Check frcons ua (frcons ub (frcons uc id)).
-    Eval compute in
-      finreduction_length
-        (frcons ua (frcons ub (frcons uc id))).
-    Eval compute in
-      finreduction_append
-        (frcons ua (frcons ub (frcons uc id)))
-        (frcons ud (frcons ue (frcons uf id))).
-End ReductionExample.
- 
+    (* Length of a finite reduction sequence *)
+    Fixpoint finreduction_length {A : ARS} {s t : @term A}
+                                 (P : finreduction t s) : nat :=
+      match P with
+      | id          => O
+      | frcons _ P' => S (finreduction_length P')
+      end.
+
+    (* Concatenation of sequences *)
+    Fixpoint finreduction_append {A : ARS} {t1 t2 t3 : @term A}
+                                 (P : finreduction t1 t2) :
+                                 finreduction t2 t3 -> finreduction t1 t3 :=
+      match P with
+      | id          => fun Q => Q
+      | frcons u P' => fun Q => frcons u (finreduction_append P' Q)
+      end.
+
+    Definition finreduction_src {A} {s t : @term A} (P : finreduction s t) : term := s.
+    Definition finreduction_tgt {A} {s t : @term A} (P : finreduction s t) : term := t.
+
+    Section ReductionExample.
+        Variable A : ARS.
+        Variable t : @term A.
+        Variable ua ub uc ud ue uf : step t t.
+        Check id.
+        Check frcons ua id.
+        Check frcons ua (frcons ub id).
+        Check frcons ua (frcons ub (frcons uc id)).
+        Eval compute in
+          finreduction_length
+            (frcons ua (frcons ub (frcons uc id))).
+        Eval compute in
+          finreduction_append
+            (frcons ua (frcons ub (frcons uc id)))
+            (frcons ud (frcons ue (frcons uf id))).
+    End ReductionExample.
+
+    Lemma finreduction_append_id_left :
+            forall {A : ARS} {t1 t2 : @term A} (P : finreduction t1 t2),
+              finreduction_append id P = P.
+      reflexivity.
+    Qed.
+
+    Lemma finreduction_append_id_right :
+            forall {A : ARS} {t1 t2 : @term A} (P : finreduction t1 t2),
+              finreduction_append P id = P.
+      intros A t1 t2 P.
+      induction P.
+      - reflexivity.
+      - simpl. rewrite IHP. reflexivity.
+    Qed.
+
+    Lemma finreduction_append_assoc :
+            forall {A : ARS} {t1 t2 t3 t4 : @term A}
+                   (P : finreduction t1 t2)
+                   (Q : finreduction t2 t3)
+                   (R : finreduction t3 t4),
+              finreduction_append (finreduction_append P Q) R =
+              finreduction_append P (finreduction_append Q R).
+      intros A t1 t2 t3 t4 P Q R.
+      induction P.
+      - reflexivity.
+      - simpl. rewrite IHP. reflexivity.
+    Qed.
+
+End FiniteReductionSequences.
+
 (* The type of steps going out from t0 *)
 Definition outgoing_step {A : ARS} (t0 : @term A) : Type := { t1 : term & step t0 t1 }.
 
@@ -106,7 +146,9 @@ Proof.
       contradiction.
 Qed.
 
-(* Deterministic Residual Structure *)
+(* Deterministic Residual Structure.
+ * We are missing the finite developments axiom, which
+ * will be treated as an extra hypothesis. *)
 Structure DRS := mkDRS {
     drs_ars : ARS ;
     drs_residual_relation : forall {t1 t2 : @term drs_ars},
@@ -141,7 +183,7 @@ Definition residual_relation_step_vs_step
     drs_residual_relation R u t3_v t4_w.
 
 Notation "s_v [ u ]¹ t_w" := (residual_relation_step_vs_step u s_v t_w)
-                               (at level 30).
+                                 (at level 30).
 
 Definition residual_set_step_vs_step
              {R : DRS} {t1 t2 : @term (drs_ars R)}
@@ -151,7 +193,8 @@ Definition residual_set_step_vs_step
     (fun t4_w : outgoing_step t2 => t3_v [ u ]¹ t4_w)
     (set_of_outgoing_steps t2).
 
-Notation "v /¹ u"   := (residual_set_step_vs_step u (existT _ _ v)) (at level 30).
+Notation "v /¹ u"   := (residual_set_step_vs_step u (existT _ _ v))
+                           (at level 30).
 
 Section ResidualStepVsStepExample.
   Variable R : DRS. 
@@ -169,7 +212,7 @@ Definition residual_set_vs_step
              {R : DRS} {t1 t2 : @term (drs_ars R)}
              (u : step t1 t2)
              (V : set (outgoing_step t1)) : set (outgoing_step t2) :=
-    set_concat_map
+    set_union_map
       (outgoing_step_dec_eq (drs_ars R) t2)
       (residual_set_step_vs_step u)
       V.
@@ -181,3 +224,181 @@ Definition residual_relation_set_vs_step
              (W : set (outgoing_step t2)) : bool :=
   set_eq (outgoing_step_dec_eq (drs_ars R) t2)
     (residual_set_vs_step u V) W.
+
+(* Residual of a multistep after a finite reduction *)
+
+Fixpoint residual_set_vs_reduction
+             {R : DRS} {t1 t2 : @term (drs_ars R)}
+             (P : finreduction t1 t2) :
+             forall V : set (outgoing_step t1), set (outgoing_step t2) :=
+  match P with                                                 
+  | id          => fun V => V
+  | frcons u P' => fun V =>
+                     residual_set_vs_reduction P' (residual_set_vs_step u V)
+  end.
+
+Definition residual_relation_set_vs_reduction
+             {R : DRS} {t1 t2 : @term (drs_ars R)}
+             (P : finreduction t1 t2)
+             (V : set (outgoing_step t1))
+             (W : set (outgoing_step t2)) : bool :=
+  set_eq (outgoing_step_dec_eq (drs_ars R) t2)
+         (residual_set_vs_reduction P V) W.
+
+(* Definition: development.
+ *
+ * Note:
+ *
+ *   The standard definition of development is stated for
+ *   both finite and infinite sequences, and then most of the
+ *   work is done assuming the finite developments theorem.
+ *
+ *   To avoid this additional complexity, we will simply
+ *   work with finite reduction sequences.
+ *)
+
+(* A reduction P is relative to a set of redexes V iff
+ * every step in P is a residual of some redex in V. *)
+Fixpoint relative_to
+             {R : DRS} {t1 t2 : @term (drs_ars R)}
+             (P : finreduction t1 t2) :
+             forall V : set (outgoing_step t1), bool :=
+  match P with
+  | id          => fun _ => true
+  | frcons u P' => fun V =>
+    andb (set_mem
+           (outgoing_step_dec_eq (drs_ars R) _)
+           (existT _ _ u)
+           V)
+         (relative_to P' (residual_set_vs_step u V))
+  end.
+
+(* A reduction PQ is relative to a set of redexes V iff
+ * P is relative to V and Q is relative to P/V. *)
+Lemma relative_to_append : forall
+             {R : DRS} {t1 t2 t3 : @term (drs_ars R)}
+             (P : finreduction t1 t2)
+             (Q : finreduction t2 t3)
+             (V : set (outgoing_step t1)),
+               relative_to (finreduction_append P Q) V =
+               andb (relative_to P V)
+                    (relative_to Q (residual_set_vs_reduction P V)).
+  intros R t1 t2 t3 P Q V.
+  induction P.
+  - reflexivity.
+  - cbn. rewrite <- Bool.andb_assoc. apply f_equal.
+    rewrite IHP. reflexivity.
+Qed.
+
+(* We say a sequence P is "right maximal" with respect to a predicate pred
+ * iff
+ * - pred holds for P and
+ * - P cannot be extended in one step in such a way that
+ *   pred also holds for the extended sequence P ++ [u]
+ * Since ARSs are assumed to be finitely branching, we may constructively
+ * check that a sequence is right maximal wrt pred.
+ *)
+Definition right_maximal_sequence
+             {A : ARS} {s t : @term A}
+             (P : finreduction s t)
+             (pred : forall t', finreduction s t' -> bool) : bool :=
+  pred t P &&
+  let steps_from_t := proj1_sig (ars_finitely_branching A t) in
+    set_forall
+      (fun t'_u =>
+         let t' := projT1 t'_u in
+         let u  := projT2 t'_u in
+           negb (pred t' (finreduction_append P (frcons u id))))
+      steps_from_t.
+
+Lemma right_maximal_sequence_correct : forall
+             {A : ARS} {s t : @term A}
+             (P : finreduction s t)
+             (pred : forall t', finreduction s t' -> bool),
+    right_maximal_sequence P pred = true ->
+    pred t P = true /\
+    forall t', forall u : step t t',
+        pred t' (finreduction_append P (frcons u id)) = false.
+  intros A s t P pred.
+  intro P_mxl.
+  unfold right_maximal_sequence in P_mxl.  
+  apply Bool.Is_true_eq_left, Bool.andb_prop_elim in P_mxl.
+  destruct P_mxl as (pred_P, no_extensions).
+  split.
+  - apply Bool.Is_true_eq_true. assumption.
+  - intros t' u.
+    apply Bool.Is_true_eq_true in no_extensions.
+    assert (no_extensions' := set_forall_correct
+                                (outgoing_step_dec_eq _ t) _ _ no_extensions).
+    specialize no_extensions' with (existT _ t' u).
+    replace false with (negb true); try reflexivity.
+    apply Bool.negb_sym. symmetry.
+    apply no_extensions'.
+    apply (proj2_sig (ars_finitely_branching A t)).
+Qed.  
+
+(* A development is a right maximal reduction relative to V. *)
+Fixpoint development
+             {R : DRS} {s t : @term (drs_ars R)}
+             (P : finreduction s t)
+             (V : set (outgoing_step s)) : bool :=
+  right_maximal_sequence P (fun _ P' => relative_to P' V).
+
+Notation "P ∝ V" := (development P V)
+                      (at level 30).
+
+(* Statement of the finite developments property *)
+
+Definition singleton_step {R : DRS} {s : @term (drs_ars R)}
+                          (t_u : outgoing_step s) : set (outgoing_step s) :=
+  set_add (outgoing_step_dec_eq _ _) t_u (empty_set _).
+
+(* If P1 and P2 develop V, then tgt(P1) = tgt(P2) *)
+Definition developments_are_cofinal :=
+       forall {R : DRS} {s : @term (drs_ars R)}
+                        (V : set (outgoing_step s))
+                        {t1 : term} (P1 : finreduction s t1)
+                        {t2 : term} (P2 : finreduction s t2),
+         P1 ∝ V = true ->
+         P2 ∝ V = true ->
+         t1 = t2.
+
+(* If P1 and P2 develop V, then u/P1 = u/P2 for all u. *)
+Definition developments_induce_same_residual_relation :=
+       forall {R : DRS} {s : @term (drs_ars R)}
+                        (V : set (outgoing_step s))
+                        {t : term} (P1 P2 : finreduction s t),
+         P1 ∝ V = true ->
+         P2 ∝ V = true ->
+         forall {t'} (u : step s t'), 
+           set_eq (outgoing_step_dec_eq _ _)
+             (residual_set_vs_reduction P1 (singleton_step (existT _ _ u)))
+             (residual_set_vs_reduction P2 (singleton_step (existT _ _ u)))
+           = true.
+
+Definition finite_developments :=
+  developments_are_cofinal /\
+  developments_induce_same_residual_relation.
+
+Definition multistep {R : DRS} {s : @term (drs_ars R)}
+                     (V : set (outgoing_step s)) : Type :=
+  { t : term & { P : finreduction s t | development P V = true } }.
+
+(* Constructively build a development, given a set of steps *)
+(**
+Definition complete_development
+       {R : DRS} {s : @term (drs_ars R)}
+       (V : set (outgoing_step s)) : multistep V :=
+**)
+(*
+ * Nope.
+ *
+ * We need König's lemma to ensure that the facts that
+ * - ARSs are finitely branching, and
+ * - developments are finite
+ * imply that
+ * - for any term, there is a bound to the length
+ *   of all complete developments starting in that term.
+ *
+ * TODO: Look for constructive alternatives to König's lemma?
+ *)
